Update IntervalTreeplus.thy

IntervalTreeplus.thy
@@ -3,60 +3,60 @@ theory IntervalTreeplus
   "Interval_Set"
 begin  
 
-fun baliL :: "'a RBs_ivl_tree \<Rightarrow> ('a ivl * 'a) \<Rightarrow> 'a RBs_ivl_tree \<Rightarrow> 'a RBs_ivl_tree" where
+fun baliL :: "'a RBs_ivl_tree ⇒ ('a ivl * 'a) ⇒ 'a RBs_ivl_tree ⇒ 'a RBs_ivl_tree" where
 "baliL (R (R t1 a t2) b t3) c t4 = R (B t1 a t2) b (B t3 c t4)" |
 "baliL (R t1 a (R t2 b t3)) c t4 = R (B t1 a t2) b (B t3 c t4)" |
 "baliL t1 a t2 = B t1 a t2"
 
-fun baliR :: "'a RBs_ivl_tree \<Rightarrow> ('a ivl * 'a) \<Rightarrow> 'a RBs_ivl_tree \<Rightarrow> 'a RBs_ivl_tree" where                                                     
+fun baliR :: "'a RBs_ivl_tree ⇒ ('a ivl * 'a) ⇒ 'a RBs_ivl_tree ⇒ 'a RBs_ivl_tree" where                                                     
 "baliR t1 a (R t2 b (R t3 c t4)) = R (B t1 a t2) b (B t3 c t4)" |
 "baliR t1 a (R (R t2 b t3) c t4) = R (B t1 a t2) b (B t3 c t4)" |
 "baliR t1 a t2 = B t1 a t2"
 
 
-fun baldL :: "('a::{linorder,order_bot}) RBs_ivl_tree \<Rightarrow> ('a ivl * 'a) \<Rightarrow> 'a RBs_ivl_tree \<Rightarrow> 'a RBs_ivl_tree" where
+fun baldL :: "('a::{linorder,order_bot}) RBs_ivl_tree ⇒ ('a ivl * 'a) ⇒ 'a RBs_ivl_tree ⇒ 'a RBs_ivl_tree" where
 "baldL (R t1 a t2) b t3 = R (B t1 a t2) b t3" |
 "baldL t1 a (B t2 b t3) = baliR t1 a (R t2 b t3)" |
 "baldL t1 a (R (B t2 b t3) c t4) = R (B t1 a t2) b (baliR t3 c (paint Red t4))" |
 "baldL t1 a t2 = R t1 a t2"
 
-fun baldR :: "('a::{linorder,order_bot}) RBs_ivl_tree \<Rightarrow> ('a ivl * 'a) \<Rightarrow> 'a RBs_ivl_tree \<Rightarrow> 'a RBs_ivl_tree" where
+fun baldR :: "('a::{linorder,order_bot}) RBs_ivl_tree ⇒ ('a ivl * 'a) ⇒ 'a RBs_ivl_tree ⇒ 'a RBs_ivl_tree" where
 "baldR t1 a (R t2 b t3) = R t1 a (B t2 b t3)" |
 "baldR (B t1 a t2) b t3 = baliL(R t1 a t2) b t3" |
 "baldR (R t1 a (B t2 b t3)) c t4 = R(baliL (paint Red t1) a t2) b (B t3 c t4)" |
 "baldR t1 a t2 = R t1 a t2"
 
-fun bheight :: "('a::{linorder,order_bot}) RBs_ivl_tree  \<Rightarrow> nat" where
+fun bheight :: "('a::{linorder,order_bot}) RBs_ivl_tree  ⇒ nat" where
 "bheight Leaf = 0" |
 "bheight (Node l (x, c) r) = (if c = Black then bheight l + 1 else bheight l)"
 
-fun invc :: " ('a::{linorder,order_bot}) RBs_ivl_tree \<Rightarrow> bool" where
+fun invc :: " ('a::{linorder,order_bot}) RBs_ivl_tree ⇒ bool" where
 "invc Leaf = True" |
 "invc (Node l (a,c) r) =
-  ((c = Red \<longrightarrow> interval_color l = Black \<and> interval_color r = Black) \<and> invc l \<and> invc r)"
+  ((c = Red ⟶ interval_color l = Black ∧ interval_color r = Black) ∧ invc l ∧ invc r)"
 
-abbreviation invc2 :: "('a::{linorder,order_bot}) RBs_ivl_tree  \<Rightarrow> bool" where
-"invc2 t \<equiv> invc(paint Black t)"
+abbreviation invc2 :: "('a::{linorder,order_bot}) RBs_ivl_tree  ⇒ bool" where
+"invc2 t ≡ invc(paint Black t)"
 
-fun invh :: "('a::{linorder,order_bot}) RBs_ivl_tree  \<Rightarrow> bool" where
+fun invh :: "('a::{linorder,order_bot}) RBs_ivl_tree  ⇒ bool" where
  "invh Leaf = True" |                                      
- "invh (Node l (x, c) r) = (bheight l = bheight r \<and> invh l \<and> invh r)"
+ "invh (Node l (x, c) r) = (bheight l = bheight r ∧ invh l ∧ invh r)"
 
 definition empty :: "'a RBs_ivl_tree" where "empty = Leaf"
 
-fun ins :: "'a::{linorder,order_bot} ivl \<Rightarrow> 'a RBs_ivl_tree \<Rightarrow> 'a RBs_ivl_tree" 
+fun ins :: "'a::{linorder,order_bot} ivl ⇒ 'a RBs_ivl_tree ⇒ 'a RBs_ivl_tree" 
   where
 "ins x Leaf = R Leaf (x,high x) Leaf" |
 "ins x (B l (a,m) r) =
   (case cmp x a of
-     LT \<Rightarrow> (baliL (ins x l) (a,m) r) |
-     GT \<Rightarrow> (baliR l (a,m) (ins x r)) |
-     EQ \<Rightarrow> B l (a,m) r)" |
+     LT ⇒ (baliL (ins x l) (a,m) r) |
+     GT ⇒ (baliR l (a,m) (ins x r)) |
+     EQ ⇒ B l (a,m) r)" |
 "ins x (R l (a,m) r) =
   (case cmp x a of
-    LT \<Rightarrow> (R (ins x l) (a,m) r) |
-    GT \<Rightarrow> (R l (a,m) (ins x r)) |
-    EQ \<Rightarrow> R l (a,m) r)"
+    LT ⇒ (R (ins x l) (a,m) r) |
+    GT ⇒ (R l (a,m) (ins x r)) |
+    EQ ⇒ R l (a,m) r)"
 
 (*
 export_code ins in Go
@@ -65,61 +65,61 @@ code_deps ins
 code_thms ins 
 code_printing ins in Haskell 
 *)
-definition insert_IntervalT::"'a::{linorder,order_bot} ivl \<Rightarrow> 'a RBs_ivl_tree \<Rightarrow> 'a RBs_ivl_tree" 
+definition insert_IntervalT::"'a::{linorder,order_bot} ivl ⇒ 'a RBs_ivl_tree ⇒ 'a RBs_ivl_tree" 
   where"insert_IntervalT x t = node (paint Black (ins x t))"
 
-fun split_min :: "'a::{linorder,order_bot} RBs_ivl_tree \<Rightarrow> (('a ivl*'a) * 'a RBs_ivl_tree)" where
+fun split_min :: "'a::{linorder,order_bot} RBs_ivl_tree ⇒ (('a ivl*'a) * 'a RBs_ivl_tree)" where
 "split_min (Node l ((a, m),_)  r) =
   (if l = Leaf then ((a,m),r)
    else let (x,l') = split_min l 
          in (x, if interval_color l = Black then baldL l' (a,m) r else R l' (a,m) r))"
 
 
-fun del :: "'a::{linorder,order_bot} ivl \<Rightarrow> 'a RBs_ivl_tree \<Rightarrow> 'a RBs_ivl_tree" where
+fun del :: "'a::{linorder,order_bot} ivl ⇒ 'a RBs_ivl_tree ⇒ 'a RBs_ivl_tree" where
 "del x Leaf = Leaf" |
 "del x (Node l ((a, m),_) r) =
   (case cmp x a of
-      LT \<Rightarrow> let l' = del x l in if l \<noteq> Leaf \<and> interval_color l = Black
+      LT ⇒ let l' = del x l in if l ≠ Leaf ∧ interval_color l = Black
             then baldL l' (a,m) r else R l' (a,m) r  |
-      GT \<Rightarrow> let r' = del x r in if r\<noteq> Leaf \<and> interval_color r = Black
+      GT ⇒ let r' = del x r in if r≠ Leaf ∧ interval_color r = Black
             then baldR l (a,m) r' else R l (a,m) r'  |
-      EQ \<Rightarrow> if r = Leaf then l else let ((a',m'),r') = split_min r in
+      EQ ⇒ if r = Leaf then l else let ((a',m'),r') = split_min r in
             if interval_color r = Black 
             then baldR l (a',m') r' else R l (a',m') r') "
  
-definition delete_IntervalT::"'a::{linorder,order_bot} ivl \<Rightarrow> 'a RBs_ivl_tree \<Rightarrow> 'a RBs_ivl_tree"  
+definition delete_IntervalT::"'a::{linorder,order_bot} ivl ⇒ 'a RBs_ivl_tree ⇒ 'a RBs_ivl_tree"  
 where "delete_IntervalT x t = node (paint Black (del x t))"
 
-fun search :: "'a::{linorder,order_bot} RBs_ivl_tree \<Rightarrow> 'a ivl \<Rightarrow> bool" where
+fun search :: "'a::{linorder,order_bot} RBs_ivl_tree ⇒ 'a ivl ⇒ bool" where
 "search Leaf x = False" |
 "search (Node l ((a,_),_) r) x =
   (if overlap x a then True
-   else if l \<noteq> Leaf \<and> max_hi l \<ge> low x then search l x
+   else if l ≠ Leaf ∧ max_hi l ≥ low x then search l x
    else search r x)"
 
-definition inv_bst::"('a::{linorder,order_bot}) RBs_ivl_tree \<Rightarrow> bool" 
-  where "inv_bst t \<equiv> sorted(inorder t)"
+definition inv_bst::"('a::{linorder,order_bot}) RBs_ivl_tree ⇒ bool" 
+  where "inv_bst t ≡ sorted(inorder t)"
 
-fun inv_color::"'a::{linorder,order_bot} RBs_ivl_tree \<Rightarrow> bool"
+fun inv_color::"'a::{linorder,order_bot} RBs_ivl_tree ⇒ bool"
   where"inv_color t = (interval_color t = Black)"
 
-definition invar_BItree :: "('a::{linorder,order_bot}) RBs_ivl_tree \<Rightarrow> bool" 
-  where" invar_BItree t = (inv_max_hi t \<and> inv_bst t \<and>invc t \<and> invh t \<and> inv_color t)"
+definition invar_BItree :: "('a::{linorder,order_bot}) RBs_ivl_tree ⇒ bool" 
+  where" invar_BItree t = (inv_max_hi t ∧ inv_bst t ∧invc t ∧ invh t ∧ inv_color t)"
                                                                      
-fun isin_IntervalT :: "'a::{linorder,order_bot} RBs_ivl_tree \<Rightarrow> 'a ivl \<Rightarrow> bool" where
+fun isin_IntervalT :: "'a::{linorder,order_bot} RBs_ivl_tree ⇒ 'a ivl ⇒ bool" where
 "isin_IntervalT Leaf x = False" |
 "isin_IntervalT (Node l ((a,_),_) r) x =
   (case cmp x a of
-     LT \<Rightarrow> isin_IntervalT l x |
-     EQ \<Rightarrow> True |
-     GT \<Rightarrow> isin_IntervalT r x)"
+     LT ⇒ isin_IntervalT l x |
+     EQ ⇒ True |
+     GT ⇒ isin_IntervalT r x)"
 
 lemma max_hi_is_max:
-  "inv_max_hi t \<Longrightarrow>  a \<in> set_tree t \<Longrightarrow> high a \<le> max_hi t"
+  "inv_max_hi t ⟹  a ∈ set_tree t ⟹ high a ≤ max_hi t"
   by(induct t, auto simp add: max3_def max_def)
 
 lemma max_hi_exists:
-  "inv_max_hi t \<Longrightarrow> t \<noteq> Leaf \<Longrightarrow> \<exists>a\<in>set_tree t. high a = max_hi t"
+  "inv_max_hi t ⟹ t ≠ Leaf ⟹ ∃a∈set_tree t. high a = max_hi t"
   apply(induct t )
   apply simp
   apply(auto simp add: max3_def max_def le_bot)
@@ -148,7 +148,7 @@ lemma inorder_baliR:
   by auto
 
 lemma inorder_ins:
-  "sorted(inorder t) \<Longrightarrow> inorder(ins x t) = ins_list x (inorder t)"
+  "sorted(inorder t) ⟹ inorder(ins x t) = ins_list x (inorder t)"
   apply(induction x t rule: ins.induct)
   by(auto simp: ins_list_simps inorder_baliL inorder_baliR)
 
@@ -161,25 +161,25 @@ lemma set_inorder[simp]: "set (inorder t) = set_tree t"
   apply (induction t)
   by auto
 
-subsubsection \<open>Isin Functional Correctness Proofs\<close>
-lemma isin_set_inorder: "sorted(inorder t) \<Longrightarrow> isin_IntervalT t x = (x \<in> set(inorder t))"
+subsubsection ‹Isin Functional Correctness Proofs›
+lemma isin_set_inorder: "sorted(inorder t) ⟹ isin_IntervalT t x = (x ∈ set(inorder t))"
   apply(induct t)
   apply(auto simp: isin_simps)
   apply (meson cmp_def)
   by auto
 
 lemma inorder_insert:
-  "sorted(inorder t) \<Longrightarrow> inorder(insert_IntervalT x t) = ins_list x (inorder t)"
+  "sorted(inorder t) ⟹ inorder(insert_IntervalT x t) = ins_list x (inorder t)"
   by (auto simp add: insert_IntervalT_def inorder_ins inorder_paint inorder_node)
 
-subsubsection \<open>Delete Functional Correctness Proofs\<close>
+subsubsection ‹Delete Functional Correctness Proofs›
 
 lemma inorder_baldL:"inorder (baldL l (a,m) r) = inorder l @ a # inorder r"
   apply(cases "(l,(a,m),r)" rule: baldL.cases)
   by (auto simp add: inorder_baliR inorder_paint)
 
 lemma split_minD:
-  "split_min t = ((a,m),t') \<Longrightarrow> t \<noteq> Leaf \<Longrightarrow> a # inorder t' = inorder t"
+  "split_min t = ((a,m),t') ⟹ t ≠ Leaf ⟹ a # inorder t' = inorder t"
   apply(induction t arbitrary: t' rule: split_min.induct)
   by(auto simp: inorder_baldL sorted_lems split: prod.splits if_splits)
  
@@ -190,7 +190,7 @@ lemma inorder_baldR:"inorder (baldR l (a, m) r) = inorder l @ a # inorder r"
   using inorder_paint by auto
 
 lemma inorder_del:
- "sorted(inorder t) \<Longrightarrow>  inorder(delete_IntervalT x t) = del_list x (inorder t)"
+ "sorted(inorder t) ⟹  inorder(delete_IntervalT x t) = del_list x (inorder t)"
   apply(simp add:delete_IntervalT_def)
   apply(induction x t rule: del.induct)
   apply(auto simp: del_list_simps inorder_baldL inorder_baldR split_minD split: prod.splits)
@@ -206,17 +206,17 @@ lemma inorder_del:
 
 subsection "Insert and Delete Inv_Max Proofs"
 lemma inv_max_hi_insert:
-  "inv_max_hi t \<Longrightarrow> inv_max_hi (insert_IntervalT x t)"
+  "inv_max_hi t ⟹ inv_max_hi (insert_IntervalT x t)"
   apply(simp add:insert_IntervalT_def )
   by (simp add: node_correct)
 
 lemma inv_max_hi_delete:
-  "inv_max_hi t \<Longrightarrow> inv_max_hi (delete_IntervalT x t)"
+  "inv_max_hi t ⟹ inv_max_hi (delete_IntervalT x t)"
   apply(simp add:delete_IntervalT_def)
   by (simp add: node_correct)
 
 lemma search_correct:
-  "inv_max_hi t \<and> sorted(inorder t) \<Longrightarrow> search t x = has_overlap (set_tree t) x"
+  "inv_max_hi t ∧ sorted(inorder t) ⟹ search t x = has_overlap (set_tree t) x"
   apply(induct t rule: tree2_induct)
   apply(auto simp : has_overlap_def overlap_def)
   apply(metis UnCI sorted_cons sorted_wrt_append)
@@ -232,13 +232,13 @@ lemma search_correct:
   apply(metis sorted_cons sorted_mid_iff)
   by(metis sorted_cons sorted_mid_iff)
 
-subsection \<open>RB Structural invariants\<close>
-subsection \<open>Insert invariants\<close>
+subsection ‹RB Structural invariants›
+subsection ‹Insert invariants›
 
-lemma neq_Black[simp]: "(c \<noteq> Black) = (c = Red)"
+lemma neq_Black[simp]: "(c ≠ Black) = (c = Red)"
   by (cases c) auto
 
-lemma invc2I: "invc t \<Longrightarrow> invc2 t"
+lemma invc2I: "invc t ⟹ invc2 t"
   apply (cases t rule: tree2_cases)
   by auto
 
@@ -248,58 +248,58 @@ lemma color_paint_Black: "interval_color  (paint Black t) = Black"
 lemma paininvh_node: "paint c2 (paint c1 t) = paint c2 t"
  by (cases t) auto
 
-lemma invh_paint: "invh t \<Longrightarrow> invh (paint c t)"
+lemma invh_paint: "invh t ⟹ invh (paint c t)"
  by (cases t) auto
 
 lemma invc_baliL:
-  "\<lbrakk>invc2 l; invc r\<rbrakk> \<Longrightarrow> invc (baliL l a r)" 
+  "⟦invc2 l; invc r⟧ ⟹ invc (baliL l a r)" 
  by (induct l a r rule: baliL.induct) auto
 
 lemma invc_baliR:
-  "\<lbrakk>invc l; invc2 r\<rbrakk> \<Longrightarrow> invc (baliR l a r)" 
+  "⟦invc l; invc2 r⟧ ⟹ invc (baliR l a r)" 
  by (induct l a r rule: baliR.induct) auto
 
 lemma bheight_baliL:
-  "bheight l = bheight r \<Longrightarrow> bheight (baliL l a r) = Suc (bheight l)"
+  "bheight l = bheight r ⟹ bheight (baliL l a r) = Suc (bheight l)"
  by (induct l a r rule: baliL.induct) auto
 
 lemma bheight_baliR:
-  "bheight l = bheight r \<Longrightarrow> bheight (baliR l a r) = Suc (bheight l)"
+  "bheight l = bheight r ⟹ bheight (baliR l a r) = Suc (bheight l)"
  by (induct l a r rule: baliR.induct) auto
 
 lemma invh_baliL: 
-  "\<lbrakk> invh l; invh r; bheight l = bheight r \<rbrakk> \<Longrightarrow> invh (baliL l a r)"
+  "⟦ invh l; invh r; bheight l = bheight r ⟧ ⟹ invh (baliL l a r)"
  by (induct l a r rule: baliL.induct) auto
 
 lemma invh_baliR: 
-  "\<lbrakk> invh l; invh r; bheight l = bheight r \<rbrakk> \<Longrightarrow> invh (baliR l a r)"
+  "⟦ invh l; invh r; bheight l = bheight r ⟧ ⟹ invh (baliR l a r)"
  by (induct l a r rule: baliR.induct) auto
 
-lemma inv_baliR: "\<lbrakk> invh l; invh r; invc l; invc2 r; bheight l = bheight r \<rbrakk>
- \<Longrightarrow> invc (baliR l a r) \<and> invh (baliR l a r) \<and> bheight (baliR l a r) = Suc (bheight l)"
+lemma inv_baliR: "⟦ invh l; invh r; invc l; invc2 r; bheight l = bheight r ⟧
+ ⟹ invc (baliR l a r) ∧ invh (baliR l a r) ∧ bheight (baliR l a r) = Suc (bheight l)"
  by (induct l a r rule: baliR.induct) auto
 
-lemma inv_baliL: "\<lbrakk> invh l; invh r; invc2 l; invc r; bheight l = bheight r \<rbrakk>
- \<Longrightarrow> invc (baliL l a r) \<and> invh (baliL l a r) \<and> bheight (baliL l a r) = Suc (bheight l)"
+lemma inv_baliL: "⟦ invh l; invh r; invc2 l; invc r; bheight l = bheight r ⟧
+ ⟹ invc (baliL l a r) ∧ invh (baliL l a r) ∧ bheight (baliL l a r) = Suc (bheight l)"
  by (induct l a r rule: baliL.induct) auto
 
-subsubsection \<open>Insertion\<close>
+subsubsection ‹Insertion›
 
-lemma invc_ins: "invc t \<longrightarrow> invc2 (ins x t) \<and> (interval_color t = Black \<longrightarrow> invc (ins x t))"
+lemma invc_ins: "invc t ⟶ invc2 (ins x t) ∧ (interval_color t = Black ⟶ invc (ins x t))"
   apply (induct x t rule: ins.induct) 
   by(auto simp: invc_baliL invc_baliR invc2I)
 
-lemma invh_ins: "invh t \<Longrightarrow> invh (ins x t) \<and> bheight (ins x t) = bheight t"
+lemma invh_ins: "invh t ⟹ invh (ins x t) ∧ bheight (ins x t) = bheight t"
   apply(induct x t rule: ins.induct)
   by(auto simp: invh_baliL invh_baliR bheight_baliL bheight_baliR)
 
-lemma inv_ins: "\<lbrakk> invc t; invh t \<rbrakk> \<Longrightarrow>
-  invc2 (ins x t) \<and> (interval_color t = Black \<longrightarrow> invc (ins x t)) \<and>
-  invh(ins x t) \<and> bheight (ins x t) = bheight t"
+lemma inv_ins: "⟦ invc t; invh t ⟧ ⟹
+  invc2 (ins x t) ∧ (interval_color t = Black ⟶ invc (ins x t)) ∧
+  invh(ins x t) ∧ bheight (ins x t) = bheight t"
   apply(induct x t rule: ins.induct) 
   by(auto simp: inv_baliL inv_baliR invc2I)
 
-lemma invc_node:"invc t \<Longrightarrow> invc(node t)"
+lemma invc_node:"invc t ⟹ invc(node t)"
   apply(induct t)
   apply (auto simp:Let_def)
   apply (metis (no_types, lifting) interval_color.elims interval_color.simps(2) node.simps(1) node.simps(2))
@@ -309,12 +309,12 @@ lemma bheight_node:"bheight t = bheight(node t)"
   apply(induct t)
   by(auto simp:Let_def) 
 
-lemma invh_node:"invh t \<Longrightarrow> invh(node t)"
+lemma invh_node:"invh t ⟹ invh(node t)"
   apply(induct t)
   apply(auto simp:Let_def )
   by(metis bheight_node)
   
-lemma inv_node:"invar_BItree t \<Longrightarrow> invar_BItree (node t)"
+lemma inv_node:"invar_BItree t ⟹ invar_BItree (node t)"
   apply(induct t)
   apply (auto simp :invar_BItree_def)
   apply (metis node_correct inv_max_hi.simps(2))
@@ -323,60 +323,60 @@ lemma inv_node:"invar_BItree t \<Longrightarrow> invar_BItree (node t)"
   apply (metis invh.simps(2) bheight_node invh_node)
   by (meson interval_color.simps(2))
 
-lemma ins_color_node:"interval_color (paint Black (ins x t)) = Black \<Longrightarrow> interval_color (node (paint Black (ins x t))) = Black"
+lemma ins_color_node:"interval_color (paint Black (ins x t)) = Black ⟹ interval_color (node (paint Black (ins x t))) = Black"
   apply(induct t)
    apply (auto simp:Let_def)
   by (metis interval_color.elims interval_color.simps(2) node.simps(1) node.simps(2))
 
-lemma del_color_node:"interval_color (paint Black (del x t)) = Black \<Longrightarrow> interval_color (node (paint Black (del x t))) = Black"
+lemma del_color_node:"interval_color (paint Black (del x t)) = Black ⟹ interval_color (node (paint Black (del x t))) = Black"
   apply(induct t)
   apply simp
   by (metis interval_color.elims interval_color.simps(2) node.simps(1) node.simps(2))
   
-subsection \<open>Delete invariants\<close>
+subsection ‹Delete invariants›
 
 lemma bheight_paint_Red:
-  "interval_color t = Black \<Longrightarrow> bheight (paint Red t) = bheight t - 1"
+  "interval_color t = Black ⟹ bheight (paint Red t) = bheight t - 1"
 by (cases t) auto
 
 lemma invh_baldL_invc:
-  "\<lbrakk> invh l;  invh r;  bheight l + 1 = bheight r;  invc r \<rbrakk>
-   \<Longrightarrow> invh (baldL l a r) \<and> bheight (baldL l a r) = bheight r"
+  "⟦ invh l;  invh r;  bheight l + 1 = bheight r;  invc r ⟧
+   ⟹ invh (baldL l a r) ∧ bheight (baldL l a r) = bheight r"
   apply(induct l a r rule: baldL.induct)
   by(auto simp: invh_baliR invh_paint bheight_baliR bheight_paint_Red)
 
 lemma invh_baldL_Black: 
-  "\<lbrakk> invh l;  invh r;  bheight l + 1 = bheight r;  interval_color r = Black \<rbrakk>
-   \<Longrightarrow> invh (baldL l a r) \<and> bheight (baldL l a r) = bheight r"
+  "⟦ invh l;  invh r;  bheight l + 1 = bheight r;  interval_color r = Black ⟧
+   ⟹ invh (baldL l a r) ∧ bheight (baldL l a r) = bheight r"
   apply(induct l a r rule: baldL.induct) 
   by(auto simp add: invh_baliR bheight_baliR) 
 
-lemma invc_baldL: "\<lbrakk>invc2 l; invc r; interval_color r = Black\<rbrakk> \<Longrightarrow> invc (baldL l a r)"
+lemma invc_baldL: "⟦invc2 l; invc r; interval_color r = Black⟧ ⟹ invc (baldL l a r)"
   apply(induct l a r rule: baldL.induct) 
   by(auto simp add: invc_baliR)
 
-lemma invc2_baldL: "\<lbrakk> invc2 l; invc r \<rbrakk> \<Longrightarrow> invc2 (baldL l a r)"
+lemma invc2_baldL: "⟦ invc2 l; invc r ⟧ ⟹ invc2 (baldL l a r)"
   apply(induct l a r rule: baldL.induct) 
   by(auto simp: invc_baliR paininvh_node invc2I)
 
 lemma invh_baldR_invc:
-  "\<lbrakk> invh l;  invh r;  bheight l = bheight r + 1;  invc l \<rbrakk>
-  \<Longrightarrow> invh (baldR l a r) \<and> bheight (baldR l a r) = bheight l"
+  "⟦ invh l;  invh r;  bheight l = bheight r + 1;  invc l ⟧
+  ⟹ invh (baldR l a r) ∧ bheight (baldR l a r) = bheight l"
   apply(induct l a r rule: baldR.induct)
   by(auto simp: invh_baliL bheight_baliL invh_paint bheight_paint_Red)
  
-lemma invc_baldR: "\<lbrakk>invc l; invc2 r; interval_color l = Black\<rbrakk> \<Longrightarrow> invc (baldR l a r)"
+lemma invc_baldR: "⟦invc l; invc2 r; interval_color l = Black⟧ ⟹ invc (baldR l a r)"
   apply(induct l a r rule: baldR.induct) 
   by(auto simp add: invc_baliL)
 
-lemma invc2_baldR: "\<lbrakk> invc l; invc2 r \<rbrakk> \<Longrightarrow>invc2 (baldR l a r)"
+lemma invc2_baldR: "⟦ invc l; invc2 r ⟧ ⟹invc2 (baldR l a r)"
   apply(induct l a r rule: baldR.induct) 
   by(auto simp: invc_baliL paininvh_node invc2I)
 
 lemma inv_baldL:
-  "\<lbrakk> invh l;  invh r;  bheight l + 1 = bheight r; invc2 l; invc r \<rbrakk>
-   \<Longrightarrow> invh (baldL l a r) \<and> bheight (baldL l a r) = bheight r
-  \<and> invc2 (baldL l a r) \<and> (interval_color r = Black \<longrightarrow> invc (baldL l a r))"
+  "⟦ invh l;  invh r;  bheight l + 1 = bheight r; invc2 l; invc r ⟧
+   ⟹ invh (baldL l a r) ∧ bheight (baldL l a r) = bheight r
+  ∧ invc2 (baldL l a r) ∧ (interval_color r = Black ⟶ invc (baldL l a r))"
   apply(induct l a r rule: baldL.induct)
   apply auto[1]
   using invc2_baldL invc_baldL invh_baldL_invc apply blast
@@ -386,9 +386,9 @@ lemma inv_baldL:
   by auto
 
 lemma inv_baldR:
-  "\<lbrakk> invh l;  invh r;  bheight l = bheight r + 1; invc l; invc2 r \<rbrakk>
-   \<Longrightarrow> invh (baldR l a r) \<and> bheight (baldR l a r) = bheight l
-  \<and> invc2 (baldR l a r) \<and> (interval_color l = Black \<longrightarrow> invc (baldR l a r))"
+  "⟦ invh l;  invh r;  bheight l = bheight r + 1; invc l; invc2 r ⟧
+   ⟹ invh (baldR l a r) ∧ bheight (baldR l a r) = bheight l
+  ∧ invc2 (baldR l a r) ∧ (interval_color l = Black ⟶ invc (baldR l a r))"
   apply(induct l a r rule: baldR.induct)
   apply force
   using invc2_baldR invc_baldR invh_baldR_invc apply blast
@@ -397,17 +397,17 @@ lemma inv_baldR:
   apply (meson invc2_baldR invc_baldR invh_baldR_invc)
   by auto
 
-lemma neq_LeafD: "t \<noteq> Leaf \<Longrightarrow> \<exists>l x c r. t = Node l (x,c) r"
+lemma neq_LeafD: "t ≠ Leaf ⟹ ∃l x c r. t = Node l (x,c) r"
   by(cases t rule: tree2_cases) auto
 
-subsection \<open>Structural invariants\<close>
-lemma neq_Red[simp]: "(c \<noteq> Red) = (c = Black)"
+subsection ‹Structural invariants›
+lemma neq_Red[simp]: "(c ≠ Red) = (c = Black)"
  by (cases c) auto
 
-lemma inv_split_min: "\<lbrakk> split_min t = (x,t'); t \<noteq> Leaf; invh t; invc t \<rbrakk> \<Longrightarrow>
-   invh t' \<and>
-   (interval_color t = Red \<longrightarrow> bheight t' = bheight t \<and> invc t') \<and>
-   (interval_color t = Black \<longrightarrow> bheight t' = bheight t - 1 \<and> invc2 t')"
+lemma inv_split_min: "⟦ split_min t = (x,t'); t ≠ Leaf; invh t; invc t ⟧ ⟹
+   invh t' ∧
+   (interval_color t = Red ⟶ bheight t' = bheight t ∧ invc t') ∧
+   (interval_color t = Black ⟶ bheight t' = bheight t - 1 ∧ invc2 t')"
   apply(induction t arbitrary: x t' rule: split_min.induct)
   apply(auto simp: inv_baldR inv_baldL invc2I  dest!: neq_LeafD)
   apply(auto split!: prod.splits if_splits)
@@ -421,74 +421,76 @@ lemma inv_split_min: "\<lbrakk> split_min t = (x,t'); t \<noteq> Leaf; invh t; i
   apply (metis Suc_eq_plus1 Suc_pred bheight.elims interval_color.simps(2) invh_baldL_Black not_gr_zero old.prod.exhaust zero_eq_add_iff_both_eq_0 zero_neq_one)
   by (auto simp add: invc2_baldL invc2I)
 
-lemma inv_del: "\<lbrakk> invh t; invc t \<rbrakk> \<Longrightarrow>
-   invh (del x t) \<and>
-   (interval_color t = Red \<longrightarrow> bheight (del x t) = bheight t \<and> invc (del x t)) \<and>
-   (interval_color t = Black \<longrightarrow> bheight (del x t) = bheight t - 1 \<and> invc2 (del x t))"
+lemma inv_del: "⟦ invh t; invc t ⟧ ⟹
+   invh (del x t) ∧
+   (interval_color t = Red ⟶ bheight (del x t) = bheight t ∧ invc (del x t)) ∧
+   (interval_color t = Black ⟶ bheight (del x t) = bheight t - 1 ∧ invc2 (del x t))"
   apply (induction x t rule: del.induct)
   by(auto simp: inv_baldR inv_baldL invc2I Let_def  
      dest!: inv_split_min 
       dest: neq_LeafD 
         split!: prod.splits if_splits)
 
-theorem set_isin:"invar_BItree t \<Longrightarrow> isin_IntervalT t x = (x \<in> set_tree t)"
+theorem set_isin:"invar_BItree t ⟹ isin_IntervalT t x = (x ∈ set_tree t)"
   by (simp add: isin_set_inorder inv_bst_def invar_BItree_def)
 
-theorem set_insert:"invar_BItree t \<Longrightarrow>set_tree (insert_IntervalT x t) = set_tree t \<union> {x}"
+theorem set_insert:"invar_BItree t ⟹set_tree (insert_IntervalT x t) = set_tree t ∪ {x}"
   apply(simp add:invar_BItree_def inv_bst_def)
   by(simp add: inorder_insert set_ins_list flip: set_inorder)
 
-theorem set_delete:"invar_BItree t \<Longrightarrow>set_tree (delete_IntervalT x t) = set_tree t - {x}"
-   apply(simp add:invar_BItree_def inv_bst_def)
-  by(simp add: inorder_del set_del_list flip: set_inorder)
+theorem set_delete:"invar_BItree t ⟹set_tree (delete_IntervalT x t) = set_tree t - {x}"
+  apply(simp add:invar_BItree_def )
+  by(simp add: inorder_del set_del_list inv_bst_def flip: set_inorder)
 
-lemma insert_max_hi:"inv_max_hi t \<Longrightarrow>inv_bst t \<Longrightarrow>invc t \<Longrightarrow> invh t 
-        \<Longrightarrow> interval_color t = Black \<Longrightarrow> inv_max_hi (node (paint Black (ins x t)))"
+
+
+lemma insert_max_hi:"inv_max_hi t ⟹inv_bst t ⟹invc t ⟹ invh t 
+        ⟹ interval_color t = Black ⟹ inv_max_hi (node (paint Black (ins x t)))"
   by (simp add: node_correct)
-lemma insert_bst:"inv_max_hi t \<Longrightarrow>inv_bst t \<Longrightarrow>invc t \<Longrightarrow> invh t 
-                    \<Longrightarrow> interval_color t = Black \<Longrightarrow> inv_bst (node (paint Black (ins x t)))"
+lemma insert_bst:"inv_max_hi t ⟹inv_bst t ⟹invc t ⟹ invh t 
+                    ⟹ interval_color t = Black ⟹ inv_bst (node (paint Black (ins x t)))"
   by(simp add:inorder_ins inorder_node inorder_paint sorted_ins_list inv_bst_def)
-lemma insert_invc:"inv_max_hi t \<Longrightarrow>inv_bst t \<Longrightarrow>invc t \<Longrightarrow> invh t 
-                    \<Longrightarrow> interval_color t = Black \<Longrightarrow> invc (node (paint Black (ins x t)))"
+lemma insert_invc:"inv_max_hi t ⟹inv_bst t ⟹invc t ⟹ invh t 
+                    ⟹ interval_color t = Black ⟹ invc (node (paint Black (ins x t)))"
   by(simp add: invc_ins invc_node)
-lemma insert_invh:"inv_max_hi t \<Longrightarrow>inv_bst t \<Longrightarrow>invc t \<Longrightarrow> invh t 
-    \<Longrightarrow> interval_color t = Black \<Longrightarrow> invh (node (paint Black (ins x t)))"
+lemma insert_invh:"inv_max_hi t ⟹inv_bst t ⟹invc t ⟹ invh t 
+    ⟹ interval_color t = Black ⟹ invh (node (paint Black (ins x t)))"
   by(simp add: inv_ins invh_node invh_paint)
-lemma insert_interval_color:"inv_max_hi t \<Longrightarrow>inv_bst t \<Longrightarrow>invc t \<Longrightarrow>invh t 
-     \<Longrightarrow> interval_color t = Black \<Longrightarrow> interval_color (node (paint Black (ins x t))) = Black"
+lemma insert_interval_color:"inv_max_hi t ⟹inv_bst t ⟹invc t ⟹invh t 
+     ⟹ interval_color t = Black ⟹ interval_color (node (paint Black (ins x t))) = Black"
   by (simp add: color_paint_Black ins_color_node)
 
-theorem BIT_insert: "invar_BItree t \<Longrightarrow> invar_BItree (insert_IntervalT x t)"
+theorem BIT_insert: "invar_BItree t ⟹ invar_BItree (insert_IntervalT x t)"
  apply (auto simp add:invar_BItree_def insert_IntervalT_def)
  using insert_max_hi insert_bst insert_invc insert_invh insert_interval_color 
  by auto
 
-lemma delete_max_hi:"inv_max_hi t \<Longrightarrow>inv_bst t \<Longrightarrow>invc t \<Longrightarrow> invh t 
-      \<Longrightarrow> interval_color t = Black \<Longrightarrow> inv_max_hi (node (paint Black (del x t)))"
+lemma delete_max_hi:"inv_max_hi t ⟹inv_bst t ⟹invc t ⟹ invh t 
+      ⟹ interval_color t = Black ⟹ inv_max_hi (node (paint Black (del x t)))"
   by (simp add: node_correct)
-lemma delete_bst:"inv_max_hi t \<Longrightarrow>inv_bst t \<Longrightarrow>invc t \<Longrightarrow> invh t 
-      \<Longrightarrow> interval_color t = Black \<Longrightarrow> inv_bst (node (paint Black (del x t)))"
+lemma delete_bst:"inv_max_hi t ⟹inv_bst t ⟹invc t ⟹ invh t 
+      ⟹ interval_color t = Black ⟹ inv_bst (node (paint Black (del x t)))"
   by(metis delete_IntervalT_def inorder_del sorted_del_list inv_bst_def)
 
-lemma delete_invc:"inv_max_hi t \<Longrightarrow>inv_bst t \<Longrightarrow>invc t \<Longrightarrow> invh t 
-       \<Longrightarrow> interval_color t = Black \<Longrightarrow> invc (node (paint Black (del x t)))"
+lemma delete_invc:"inv_max_hi t ⟹inv_bst t ⟹invc t ⟹ invh t 
+       ⟹ interval_color t = Black ⟹ invc (node (paint Black (del x t)))"
   by (simp add: inv_del invc_node)
-lemma delete_invh:"inv_max_hi t \<Longrightarrow>inv_bst t \<Longrightarrow>invc t \<Longrightarrow> invh t 
-        \<Longrightarrow> interval_color t = Black \<Longrightarrow> invh (node (paint Black (del x t)))"
+lemma delete_invh:"inv_max_hi t ⟹inv_bst t ⟹invc t ⟹ invh t 
+        ⟹ interval_color t = Black ⟹ invh (node (paint Black (del x t)))"
   by (simp add: inv_del invh_node invh_paint)
-lemma delete_interval_color:"inv_max_hi t \<Longrightarrow>inv_bst t \<Longrightarrow>invc t \<Longrightarrow>invh t 
-    \<Longrightarrow> interval_color t = Black \<Longrightarrow> interval_color (node (paint Black (del x t))) = Black"
+lemma delete_interval_color:"inv_max_hi t ⟹inv_bst t ⟹invc t ⟹invh t 
+    ⟹ interval_color t = Black ⟹ interval_color (node (paint Black (del x t))) = Black"
   by (simp add: color_paint_Black del_color_node)
 
 
-theorem BIT_delete: "invar_BItree t \<Longrightarrow> invar_BItree (delete_IntervalT x t)"
+theorem BIT_delete: "invar_BItree t ⟹ invar_BItree (delete_IntervalT x t)"
   apply(auto simp: delete_IntervalT_def invar_BItree_def)
   using delete_max_hi delete_bst delete_invc delete_invh delete_interval_color
   by auto
 
 
 theorem BIT_search:
-  "invar_BItree t\<Longrightarrow> search t x = has_overlap (set_tree t) x"
+  "invar_BItree t⟹ search t x = has_overlap (set_tree t) x"
   by (simp add: invar_BItree_def search_correct inv_bst_def)
 
 end
